formal/hol4/F4FPPVerifyEndToEndF4sGoalsScript.sml
@@ -28,11 +28,12 @@ open F4FPPVerifySMLBridgeGoalsTheory;
 open F4FPPVerifyFastProgramSplitBridgeGoalsTheory;
 open F4FPPVerifySlowBridgeDetailedGoalsTheory;
 open F4FPPVerifyRefinedMainGoalsTheory;
-open F4FPPVerifyRefinedBridgeGoalsTheory;
-open F4FPPVerifySpecTheory;
-open F4FPPBottomLayerGoalsTheory;
-open F4FPPVerifyAtlasFFIContractsGoalsTheory;
-open F4FPPVerifyAtlasEqSetGoalsTheory;
+	open F4FPPVerifyRefinedBridgeGoalsTheory;
+	open F4FPPVerifySpecTheory;
+	open F4FPPBottomLayerGoalsTheory;
+	open F4FPPBottomLayerGoalsAtlasEqTheory;
+	open F4FPPVerifyAtlasFFIContractsGoalsTheory;
+	open F4FPPVerifyAtlasEqSetGoalsTheory;
 
 val _ = new_theory "F4FPPVerifyEndToEndF4sGoals";
 
@@ -75,6 +76,26 @@ Theorem fast_and_slow_programs_succeed_gives_equivalence_atlas_eq_F4s_fast_atlas
       bottom_layer_total_ok F4s dirac (U_fast F4s)
 Proof
   metis_tac[fast_and_slow_programs_succeed_gives_refined_equivalence_atlas_eq_fast_atlas_eq]
+QED
+
+Theorem fast_and_slow_programs_succeed_gives_equivalence_atlas_eq_F4s_bottom_layer_atlas_eq:
+  !dirac.
+    atlas_hash_eq_ok /\ atlas_eq_congruent_bottom_layer /\
+    fast_program_succeeds F4s dirac /\ slow_program_succeeds F4s ==>
+      set_atlas_eq (U_fast F4s) (U_slow F4s (D_slow F4s)) /\
+      bottom_layer_total_ok_atlas_eq F4s dirac (U_fast F4s)
+Proof
+  metis_tac[fast_and_slow_programs_succeed_gives_refined_equivalence_atlas_eq_bottom_layer_atlas_eq]
+QED
+
+Theorem fast_and_slow_programs_succeed_gives_equivalence_atlas_eq_F4s_fast_atlas_eq_bottom_layer_atlas_eq:
+  !dirac.
+    atlas_hash_eq_ok /\ atlas_eq_congruent_bottom_layer /\
+    fast_program_succeeds F4s dirac /\ slow_program_succeeds F4s ==>
+      set_atlas_eq (U_fast F4s) (U_slow F4s (D_slow F4s)) /\
+      bottom_layer_total_ok_atlas_eq F4s dirac (U_fast F4s)
+Proof
+  metis_tac[fast_and_slow_programs_succeed_gives_refined_equivalence_atlas_eq_fast_atlas_eq_bottom_layer_atlas_eq]
 QED
 
 Theorem fast_and_slow_programs_succeed_gives_equivalence_atlas_eq_F4s_dirac:
